Clap/eDSLState/CircuitEvalSt.lean
@@ -1,0 +1,282 @@
+import Clap.eDSLState.Varstore
+
+import Clap.eDSLState.HashCons.Eval
+import Clap.eDSLState.HashCons.HashConsSt
+
+namespace Clap
+
+open HashConsM
+
+structure EvalSt (p : ℕ) where
+  numAlloc : ℕ
+  varStore : VarStore p
+  constraints : Prop
+  deriving Inhabited
+
+namespace EvalSt
+
+/--
+Hic sunt dracones.
+
+TODO: Nuke this
+-/
+lemma stupidext {p : ℕ} (result : EvalSt p) :
+  result = ⟨result.numAlloc, result.varStore, result.constraints⟩ := rfl
+
+section EvalSt
+
+variable {p numAlloc : ℕ} {Γ : VarStore p} {st : EvalSt p} {constraints constraint : Prop}
+
+def empty (p : ℕ) : EvalSt p := ⟨0, ∅, True⟩
+
+def unconstrained (numAlloc : ℕ) (Γ : VarStore p) : EvalSt p :=
+  ⟨numAlloc, Γ, True⟩
+
+notation
+  "unconstrained[" numAlloc:arg "]" "[" varStore:arg "]" => unconstrained numAlloc varStore
+
+@[simp, grind =]
+lemma numAlloc_unconstrained : unconstrained[numAlloc][Γ].numAlloc = numAlloc := rfl
+
+@[simp, grind =]
+lemma varStore_unconstrained : unconstrained[numAlloc][Γ].varStore = Γ := rfl
+
+@[simp, grind =]
+lemma constraints_unconstrained : unconstrained[numAlloc][Γ].constraints = True := rfl
+
+def addConstraint (st : EvalSt p) (constraint : Prop) : EvalSt p :=
+  {st with constraints := st.constraints ∧ constraint}
+
+@[simp, grind =]
+lemma addConstraint_mk
+:
+  (EvalSt.mk numAlloc Γ constraints).addConstraint constraint =
+  EvalSt.mk numAlloc Γ (constraints ∧ constraint)
+:= rfl
+
+@[simp, grind =]
+lemma addConstraint_unconstrained :
+  unconstrained[numAlloc][Γ].addConstraint constraint =
+  ⟨numAlloc, Γ, constraint⟩ := by simp [unconstrained]
+
+@[simp, grind =]
+lemma numAlloc_addConstraint : (st.addConstraint constraint).numAlloc = st.numAlloc := rfl
+
+@[simp, grind =]
+lemma varStore_addConstraint : (st.addConstraint constraint).varStore = st.varStore := rfl
+
+@[simp, grind =]
+lemma constraints_addConstraint : (st.addConstraint constraint).constraints =
+                                  (st.constraints ∧ constraint) := rfl
+
+def allocAnonymous (st : EvalSt p) : EvalSt p :=
+  {st with numAlloc := st.numAlloc + 1}
+
+@[simp, grind =]
+lemma allocAnonymous_mk
+:
+  (EvalSt.mk numAlloc Γ constraints).allocAnonymous =
+  EvalSt.mk (numAlloc + 1) Γ constraints
+:= rfl
+
+@[simp, grind =]
+lemma allocAnonymous_unconstrained :
+  unconstrained[numAlloc][Γ].allocAnonymous =
+  ⟨numAlloc + 1, Γ, True⟩ := rfl
+
+@[simp, grind =]
+lemma numAlloc_allocAnonymous : st.allocAnonymous.numAlloc = st.numAlloc + 1 := rfl
+
+@[simp, grind =]
+lemma varStore_allocAnonymous : st.allocAnonymous.varStore = st.varStore := rfl
+
+@[simp, grind =]
+lemma constraints_allocAnonymous : st.allocAnonymous.constraints = st.constraints := rfl
+
+@[grind =]
+def get? (st : EvalSt p) (e : Expr p) : Option (ZMod p) := do
+  [st.varStore|e]
+
+@[grind =]
+def getM? (st : EvalSt p) (e : HashConsM p ExprRef) : HashConsM p (Option (ZMod p)) := do
+  HashConsM.evalM st.varStore e
+
+instance : Membership (Expr p) (EvalSt p) :=
+  ⟨fun Γ e ↦ (get? Γ e).isSome⟩
+
+instance : GetElem (EvalSt p) (Expr p) (ZMod p) (fun Γ x ↦ x ∈ Γ) :=
+  ⟨fun circuitResult e h ↦ circuitResult.get? e |>.get h⟩
+
+def getD (result : EvalSt p) (e : Expr p) : ZMod p :=
+  (result.get? e).getD 0
+
+instance : GetElem? (EvalSt p) (Expr p) (ZMod p) (fun Γ x ↦ x ∈ Γ) :=
+  ⟨get?, getD⟩
+
+def getDM (result : EvalSt p) (e : HashConsM p ExprRef) : HashConsM p (ZMod p) := do
+  result.getM? e <&> Option.getD (dflt := 0)
+
+variable {e! : ExprRef} {σ : HashConsSt p} {eM : HashConsM p ExprRef} {e : Expr p}
+
+@[simp, grind =]
+lemma getD_eq_getM?_getD : st.getD e = (st[e]?).getD 0 := rfl
+
+@[simp, grind =]
+lemma getElem!_eq_getElem?_getD : st[e]! = (st[e]?).getD 0 := rfl
+
+@[simp, grind =]
+lemma getDM_eq_getM?_getD : st.getDM eM = st.getM? eM <&> Option.getD (dflt := 0) := rfl
+
+@[simp, grind =]
+lemma get?_mk
+:
+  (EvalSt.mk numAlloc Γ constraints).get? e = [Γ|e]
+:= rfl
+
+@[simp, grind =]
+lemma getM?_mk
+:
+  ((EvalSt.mk numAlloc Γ constraints).getM? eM).run σ = [Γ,σ|←eM]
+:= rfl
+
+@[simp, grind =]
+lemma getElem?_mk
+:
+  (EvalSt.mk numAlloc Γ constraints)[e]? = [Γ|e]
+:= rfl
+
+@[simp, grind =]
+lemma membership_unconstrained
+:
+  (e ∈ unconstrained[numAlloc][Γ]) = [Γ|e].isSome
+:= rfl
+
+@[simp, grind =]
+lemma getElem?_unconstrained
+:
+  unconstrained[numAlloc][Γ][e]? = [Γ|e]
+:= rfl
+
+@[simp, grind =]
+lemma getM?_unconstrained:
+  (unconstrained[numAlloc][Γ].getM? eM).run σ = [Γ,σ|←eM] := by
+  simp [unconstrained]
+
+@[grind =_]
+lemma getM?_unconstrained_eq_getM?_mk :
+  (unconstrained[numAlloc][Γ].getM? eM).run σ =
+  ((EvalSt.mk numAlloc Γ constraints).getM? eM).run σ := by grind
+
+variable {st' : EvalSt p}
+
+@[grind =>]
+lemma get?_of_varStore_eq_varStore (h : st.varStore = st'.varStore)
+:
+  st.get? e = st'.get? e
+:= by grind
+
+@[grind =>]
+lemma getElem?_of_varStore_eq_varStore (h : st.varStore = st'.varStore)
+:
+  st[e]? = st'[e]?
+:= get?_of_varStore_eq_varStore h
+
+@[grind =>]
+lemma getM?_of_varStore_eq_varStore (h : st.varStore = st'.varStore) :
+  st.getM? eM = st'.getM? eM := by
+  simp_all [EvalSt.getM?]
+
+/--
+Asserts that the expression that e points to does not use any variables that aren't in the varStore
+Panics if e is outside of σ
+-/
+def assertAllocated (st : EvalSt p) (e : Expr p) : EvalSt p :=
+  st.addConstraint st[e]?.isSome
+
+def assertAllocatedM (st : EvalSt p) (e : HashConsM p ExprRef) : HashConsM p (EvalSt p) := do
+  let val ← st.getM? e
+  return st.addConstraint val.isSome
+
+@[simp, grind =]
+lemma assertAllocated_mk
+:
+  (EvalSt.mk numAlloc Γ constraints).assertAllocated e =
+  EvalSt.mk numAlloc Γ (constraints ∧ [Γ|e].isSome)
+:= rfl
+
+@[simp, grind =]
+lemma assertAllocatedM_mk
+:
+  ((EvalSt.mk numAlloc Γ constraints).assertAllocatedM eM).run σ =
+  (
+    EvalSt.mk
+      numAlloc
+      Γ
+      (constraints ∧ [Γ,σ|←eM].1.isSome)
+    ,
+    [Γ,σ|←eM].2
+  )
+:= rfl
+
+@[simp, grind =]
+lemma numAlloc_assertAllocated :
+  (st.assertAllocated e).numAlloc = st.numAlloc := rfl
+
+@[simp, grind =]
+lemma varStore_assertAllocated :
+  (st.assertAllocated e).varStore = st.varStore := rfl
+
+@[simp, grind =]
+lemma constraints_assertAllocated :
+  (st.assertAllocated e).constraints = (st.constraints ∧ st[e]?.isSome) := rfl
+
+@[simp, grind =]
+lemma assertAllocated_unconstrained :
+  unconstrained[numAlloc][Γ].assertAllocated e =
+  letI α := unconstrained[numAlloc][Γ]
+  α.addConstraint (e ∈ α) := rfl
+
+def alloc {k p : ℕ} (result : EvalSt p) (vals : Vector (ZMod p) k) : EvalSt p :=
+  let indexed := (Vector.range k).map (·+result.numAlloc) |>.zip vals
+  let varStore := result.varStore.insertMany indexed
+  {result with varStore := varStore, numAlloc := result.numAlloc + k}
+
+@[simp, grind =]
+lemma alloc_mk
+  {k : ℕ}
+  {vals : Vector (ZMod p) k}
+:
+  (EvalSt.mk numAlloc Γ constraints).alloc vals =
+  EvalSt.mk
+    (numAlloc + k)
+    (varStore.insertMany ((Vector.range k).map (·+numAlloc) |>.zip vals))
+    constraints
+:= rfl
+
+@[simp, grind =]
+lemma numAlloc_alloc :
+  (result.alloc vars).numAlloc = result.numAlloc + k := rfl
+
+@[simp, grind =]
+lemma varStore_alloc :
+  (result.alloc vars).varStore =
+  result.varStore.insertMany ((Vector.range k).map (·+result.numAlloc) |>.zip vars) := rfl
+
+@[simp, grind =]
+lemma constraints_alloc {vars : Vector (ZMod p) k} :
+  (result.alloc vars).constraints = result.constraints := rfl
+
+def step (result : CircuitResult p) (next : Gate p) (σ : HashConsSt p) : CircuitResult p :=
+  match next with
+  | .eq0 e => result.addConstraint (result[(e, σ)]? = Option.some 0)
+  | .share e => (result.assertAllocated e σ).alloc #v[result[(e, σ)]!]
+  | .isZero e => (result.assertAllocated e σ).alloc #v[if result[(e, σ)]? = Option.some 0 then 1 else 0]
+  | .num2bits width e => (result.assertAllocated e σ).alloc (num2bitsLsbPureV width (result[(e, σ)]!))
+
+notation "[" res ", " σ "|" cmd "]ₛ" => step res cmd σ
+
+end EvalSt
+
+end EvalSt
+
+end Clap
