Clap/eDSLState/Gate.lean
@@ -1,0 +1,60 @@
+import Clap.eDSLState.HashCons.Eval
+
+namespace Clap
+
+@[grind cases]
+inductive Gate (p : ℕ) where
+  | eq0 (e : ExprRef)
+  | share (e : ExprRef)
+  | isZero (e : ExprRef)
+  | num2bits (w : ℕ) (e : ExprRef)
+deriving Inhabited
+
+namespace Gate
+
+section Gate
+
+variable {p : ℕ}
+
+@[grind =]
+def expr (gate : Gate p) : ExprRef :=
+  match gate with
+  | .eq0 e | .share e | .isZero e | .num2bits _ e => e
+
+@[grind =]
+def refsValid (gate : Gate p) (bound : ℕ) : Prop := gate.expr < bound
+
+@[grind =]
+def varsAllocated (gate : Gate p) (Γ : VarStore p) (σ : HashConsSt p) : Prop :=
+  [Γ, σ|gate.expr].isSome
+
+@[aesop safe cases, grind]
+structure wellFormed (gate : Gate p) (Γ : VarStore p) (σ : HashConsSt p) : Prop where
+  refsValid : gate.refsValid σ.size
+  varsAllocated : gate.varsAllocated Γ σ
+
+variable {gate : Gate p} {Γ : VarStore p} {σ : HashConsSt p} {e! : ExprRef} {bound : ℕ}
+
+instance : Decidable (gate.refsValid bound) :=
+  inferInstanceAs <| Decidable (gate.expr < bound)
+
+instance a : Decidable (gate.varsAllocated Γ σ) :=
+  inferInstanceAs <| Decidable ([Γ, σ|gate.expr].isSome)
+
+@[simp, grind =]
+lemma varsAllocated_eq0 : varsAllocated (.eq0 e!) Γ σ = [Γ, σ|e!].isSome := rfl
+
+@[simp, grind =]
+lemma varsAllocated_share : varsAllocated (.share e!) Γ σ = [Γ, σ|e!].isSome := rfl
+
+@[simp, grind =]
+lemma varsAllocated_isZero : varsAllocated (.isZero e!) Γ σ = [Γ, σ|e!].isSome := rfl
+
+@[simp, grind =]
+lemma varsAllocated_num2bits {w} : varsAllocated (.num2bits w e!) Γ σ = [Γ, σ|e!].isSome := rfl
+
+end Gate
+
+end Gate
+
+end Clap
